\documentclass{book}

\input{../activities-preamble.tex}
\begin{document}
\setcounter{project}{270}
\addtocounter{project}{-1}
\begin{activity}[]\label{activity-263}
\hypertarget{p-1448}{}%
Solve the recurrence \(a_n= 4a_{n-1} - 4a_{n-2}\).%
\par\smallskip%
\noindent\textbf{Solution.}\hypertarget{solution-211}{}\quad%
\hypertarget{p-1449}{}%
%
\begin{align*}
\sum_{n=2}^\infty a_nx^n  \amp=  4\sum_{n=2}^\infty a_{n-1}x^n -
4\sum_{n=2}^\infty a_{n-2}x^n\\
\sum_{n=0}^\infty a_nx^n -a_0-a_1x  \amp=  4x(\sum_{n=0}^\infty a_{n}x^n
-a_0) - 4x^2\sum_{n=0}^\infty a_{n}x^n\\
(1-4x+4x^2)\sum_{n=0}^\infty a_nx^n   \amp=
a_0+a_1x-4a_0x\\
\sum_{n=0}^\infty a_nx^n \amp= \frac{a_0+a_1x-4a_0x}{(1-4x+4x^2)}\\
\sum_{n=0}^\infty a_nx^n \amp= \frac{a_0+a_1x-4a_0x}{(1-2x)^2}\\
\sum_{n=0}^\infty a_nx^n \amp= (a_0+a_1x-4a_0x)\sum_{n=0}^\infty \binom{n+2-1}{n}
2^nx^n\\
\sum_{n=0}^\infty a_nx^n \amp= (a_0+a_1x-4a_0x)\sum_{n=0}^\infty (n+1)
2^nx^n
\end{align*}
Thus \(a_n=a_0(n+1)2^n
+(a_1-4a_0)n2^{n-1}=a_02^n+(a_1-2a_0)n2^{n-1}\).%
\end{activity}
\end{document}
