\documentclass{book}

\input{../activities-preamble.tex}
\begin{document}
\setcounter{project}{264}
\addtocounter{project}{-1}
\begin{activity}[]\label{partialfractionsintro}
\hypertarget{p-1372}{}%
In \hyperref[simplifysumoffractions]{Activity~\ref{simplifysumoffractions}} you see that when we added numerical multiples of the reciprocals of first degree polynomials we got a fraction in which the denominator is a quadratic polynomial. This will always happen unless the two denominators are multiples of each other, because their least common multiple will simply be their product, a quadratic polynomial. This leads us to ask whether a fraction whose denominator is a quadratic polynomial can always be expressed as a sum of fractions whose denominators are first degree polynomials. Find numbers \(c\) and \(d\) so that%
\begin{equation*}
\frac{5x+1}{(x-3)(x+5)} = \frac{c}{x-3} + \frac{d}{x+5}.
\end{equation*}
%
\par\smallskip%
\noindent\textbf{Hint.}\hypertarget{hint-169}{}\quad%
\hypertarget{p-1373}{}%
%
\begin{equation*}
\frac{5x+1}{(x-3)(x-5)} = \frac{cx+5c+dx-3d}{(x-3)(x-5)}
\end{equation*}
gives us%
\begin{align*}
5x \amp = cx+dx\\
1 \amp= 5c-3d\text{.}
\end{align*}
%
~\hfill{\tiny\hyperlink{a-264}{[hint]}\hypertarget{q-264}{}}\par\smallskip%
\noindent\textbf{Solution.}\hypertarget{solution-166}{}\quad%
\hypertarget{p-1374}{}%
%
\begin{align*}
\frac{5x+1}{(x-3)(x+5)}  \amp=  \frac{c}{x-3} + \frac{d}{x+5}\\
\frac{5x+1}{(x-3)(x-5)}  \amp= cx+5c+dx-3d
\end{align*}
gives us%
\begin{align*}
5x \amp= cx+dx\\
1 \amp= 5c-3d\\
5 \amp= c+d\\
1 \amp= 5c-3d
\end{align*}
This gives us \(16=8c\) so that \(c=2\) and then \(d=3\).%
\end{activity}

\clearpage\end{document}
